Intermediate/CS.v
@@ -819,7 +819,7 @@ Inductive step (G : global_env) : state -> trace event_inform -> state -> Prop :
     (* RB: TODO: [DynShare] Restore check after making it computational. *)
     (* update_reachability_of_component_with_value call_arg C' reach = reach' -> *)
     step G (gps, mem, regs, pc, addrs)
-           [ECall (Pointer.component pc) P call_arg C']
+           [ECall (Pointer.component pc) P call_arg mem C']
            (Pointer.inc pc :: gps, mem, Register.invalidate regs,
             (Permission.code, C', b, 0%Z), addrs) (* reach', replace addrs *)
 
@@ -831,7 +831,7 @@ Inductive step (G : global_env) : state -> trace event_inform -> state -> Prop :
     (* RB: TODO: [DynShare] Restore check after making it computational. *)
     (* update_reachability_of_component_with_value ret_arg (Pointer.component pc') reach = reach' -> *)
     step G (pc' :: gps', mem, regs, pc, addrs)
-           [ERet (Pointer.component pc) ret_arg (Pointer.component pc')]
+           [ERet (Pointer.component pc) ret_arg mem (Pointer.component pc')]
            (gps', mem, Register.invalidate regs, pc', addrs) (* reach', replace addrs *).
 
 Ltac step_of_executing :=
@@ -861,8 +861,8 @@ Ltac step_of_executing :=
 
 Definition event_non_inform_of (e: trace event_inform) : trace event :=
   match e with
-  | [ECall C P call_arg C'] => [CompCert.Events.ECall C P call_arg C']
-  | [ERet C v C'] => [CompCert.Events.ERet C v C']
+  | [ECall C P call_arg mem C'] => [CompCert.Events.ECall C P call_arg mem C']
+  | [ERet C v mem C'] => [CompCert.Events.ERet C v mem C']
   | _ => E0
   end.
 
@@ -1091,7 +1091,7 @@ Definition eval_step (G: global_env) (s: state) : option (trace event_inform * s
           do b <- EntryPoint.get C' P (genv_entrypoints G);
           let val := Register.get R_COM regs in
           let pc' := (Permission.code, C', b, 0%Z) in
-          let t := [ECall (Pointer.component pc) P val C'] in
+          let t := [ECall (Pointer.component pc) P val mem C'] in
           ret (t, (Pointer.inc pc :: gps, mem, Register.invalidate regs, pc', addrs))
         else
           None
@@ -1102,7 +1102,7 @@ Definition eval_step (G: global_env) (s: state) : option (trace event_inform * s
       | pc' :: gps' =>
         if negb (Component.eqb (Pointer.component pc) (Pointer.component pc')) then
           let val := Register.get R_COM regs in
-          let t := [ERet (Pointer.component pc) val (Pointer.component pc')] in
+          let t := [ERet (Pointer.component pc) val mem (Pointer.component pc')] in
           ret (t, (gps', mem, Register.invalidate regs, pc', addrs))
         else
           None
@@ -1812,8 +1812,9 @@ Fixpoint project_non_inform t_inform :=
   | [] => []
   | e :: es =>
     match e with
-    | ECall C P call_arg C' => (CompCert.Events.ECall C P call_arg C') :: project_non_inform es
-    | ERet C v C' => (CompCert.Events.ERet C v C') :: project_non_inform es
+    | ECall C P call_arg mem C' =>
+      (CompCert.Events.ECall C P call_arg mem C') :: project_non_inform es
+    | ERet C v mem C' => (CompCert.Events.ERet C v mem C') :: project_non_inform es
     | _ => project_non_inform es
     end
   end.
@@ -1894,7 +1895,7 @@ Proof.
   - simpl.
     assert (step_non_inform G (gps, mem, regs, pc, addrs)
                             (event_non_inform_of
-                               [ECall (Pointer.component pc) P call_arg C'])
+                               [ECall (Pointer.component pc) P call_arg mem C'])
                             (Pointer.inc pc :: gps, mem,
                              Register.invalidate regs,
                              (Permission.code, C', b, 0%Z), addrs)
@@ -1909,7 +1910,7 @@ Proof.
   - simpl. 
     assert (step_non_inform G (pc' :: gps', mem, regs, pc, addrs)
                             (event_non_inform_of
-                               [ERet (Pointer.component pc) ret_arg (Pointer.component pc')])
+                               [ERet (Pointer.component pc) ret_arg mem (Pointer.component pc')])
                             (gps', mem, Register.invalidate regs, pc', addrs)
            ) as gl.
     {
@@ -2206,10 +2207,10 @@ Proof.
   - match goal with Hfind: find_label_in_procedure _ ?pc ?l0 = Some ?pc' |- _ =>
                     exact (find_label_in_procedure_1 G pc pc' l0 Hfind)
     end.
-  - match goal with Hnoninf: _ = E0, He: [ECall _ _ _ _] = _ |- _ =>
+  - match goal with Hnoninf: _ = E0, He: [ECall _ _ _ _ _] = _ |- _ =>
                     rewrite <- He in Hnoninf; simpl in Hnoninf; discriminate
     end.
-  - match goal with Hnoninf: _ = E0, He: [ERet _ _ _] = _ |- _ =>
+  - match goal with Hnoninf: _ = E0, He: [ERet _ _ _ _] = _ |- _ =>
                     rewrite <- He in Hnoninf; simpl in Hnoninf; discriminate
     end.
 Qed.
@@ -2297,10 +2298,10 @@ Proof.
     + match goal with Hfind: find_label_in_procedure ?G ?pc ?l0 = Some ?pc' |- _ =>
                       rewrite <- (find_label_in_procedure_1 G pc pc' l0 Hfind)
       end. assumption.
-    + match goal with Hnoninf: _ = E0, He: [ECall _ _ _ _] = _ |- _ =>
+    + match goal with Hnoninf: _ = E0, He: [ECall _ _ _ _ _] = _ |- _ =>
                       rewrite <- He in Hnoninf; simpl in Hnoninf; discriminate
       end.
-    + match goal with Hnoninf: _ = E0, He: [ERet _ _ _] = _ |- _ =>
+    + match goal with Hnoninf: _ = E0, He: [ERet _ _ _ _] = _ |- _ =>
                       rewrite <- He in Hnoninf; simpl in Hnoninf; discriminate
       end.
 Qed.
